Cslib/Computability/Automata/NFA.lean
@@ -5,6 +5,7 @@ Authors: Fabrizio Montesi
 -/
 
 import Cslib.Computability.Automata.NA
+import Cslib.Computability.Languages.Language
 
 namespace Cslib
 
@@ -20,6 +21,8 @@ structure NFA (State : Type _) (Symbol : Type _) extends NA State Symbol where
 
 namespace NFA
 
+variable {State : Type _} {Symbol : Type _}
+
 /-- An NFA accepts a string if there is a multi-step accepting derivative with that trace from
 the start state. -/
 @[scoped grind]
@@ -28,13 +31,13 @@ def Accepts (nfa : NFA State Symbol) (xs : List Symbol) :=
 
 /-- The language of an NFA is the set of strings that it accepts. -/
 @[scoped grind]
-def language (nfa : NFA State Symbol) : Set (List Symbol) :=
+def language (nfa : NFA State Symbol) : Language Symbol :=
   { xs | nfa.Accepts xs }
 
-/-- A string is accepted by an NFA iff it is in the language of the NFA. -/
+/-- A string is in the language of an NFA iff it is accepted by the NFA. -/
 @[scoped grind =]
-theorem accepts_mem_language (nfa : NFA State Symbol) (xs : List Symbol) :
-  nfa.Accepts xs ↔ xs ∈ nfa.language := by rfl
+theorem mem_language (nfa : NFA State Symbol) (xs : List Symbol) :
+  xs ∈ nfa.language ↔ nfa.Accepts xs := Iff.rfl
 
 end NFA
 
